[pure_dB] Replaced old Store_thm calls by Theorem[simp]

examples/lambda/other-models/pure_dBScript.sml
@@ -11,8 +11,6 @@ open boolSimps arithmeticTheory pred_setTheory string_numTheory listTheory;
 
 open termTheory appFOLDLTheory chap2Theory chap3Theory;
 
-fun Store_thm(trip as (n,t,tac)) = store_thm trip before export_rewrites [n]
-
 val _ = new_theory "pure_dB"
 
 val _ = temp_set_fixity "=" (Infix(NONASSOC, 100))
@@ -23,37 +21,37 @@ val _ = Datatype`pdb = dV num | dAPP pdb pdb | dABS pdb`
 (* Definitions of lift and substitution from Nipkow's "More Church-Rosser
    proofs". NOTE: ‘lift s 0’ will forcely lift everything.
  *)
-val lift_def = Define`
+Definition lift_def :
   (lift (dV i) k = if i < k then dV i else dV (i + 1)) /\
   (lift (dAPP s t) k = dAPP (lift s k) (lift t k)) /\
   (lift (dABS s) k = dABS (lift s (k + 1)))
-`;
+End
 val _ = export_rewrites ["lift_def"]
 
 (* "Nipkow" substitution *)
-val nsub_def = Define`
+Definition nsub_def :
   (nsub s k (dV i) = if k < i then dV (i - 1)
                        else if i = k then s else dV i) /\
   (nsub s k (dAPP t u) = dAPP (nsub s k t) (nsub s k u)) /\
   (nsub s k (dABS t) = dABS (nsub (lift s 0) (k + 1) t))
-`;
+End
 val _ = export_rewrites ["nsub_def"]
 
 (* substitution that corresponds to substitution in the lambda-calculus;
    no variable decrementing in the dV clause *)
-val sub_def = Define`
+Definition sub_def :
   (sub s k (dV i) = if i = k then s else dV i) /\
   (sub s k (dAPP t u) = dAPP (sub s k t) (sub s k u)) /\
   (sub s k (dABS t) = dABS (sub (lift s 0) (k + 1) t))
-`;
+End
 val _ = export_rewrites ["sub_def"]
 
-Overload SUB = “sub” (* same syntax as SUB *)
+Overload SUB = “sub” (* same [./.] syntax as SUB *)
 
 (* a variable-binding lambda-equivalent for dB terms *)
-val dLAM_def = Define`
+Definition dLAM_def :
   dLAM v body = dABS (sub (dV 0) (v + 1) (lift body 0))
-`
+End
 
 (* the set of free indices in a term *)
 val dFV_def = Define`
@@ -962,34 +960,37 @@ val toTerm_def = new_specification(
 val fromtoTerm = save_thm("fromtoTerm", GSYM toTerm_def)
 val _ = export_rewrites ["fromtoTerm"]
 
-val toTerm_11 = Store_thm(
-  "toTerm_11",
-  ``(toTerm d1 = toTerm d2) <=> (d1 = d2)``,
+Theorem toTerm_11[simp] :
+    (toTerm d1 = toTerm d2) <=> (d1 = d2)
+Proof
   SRW_TAC [][EQ_IMP_THM] THEN
   POP_ASSUM (MP_TAC o Q.AP_TERM `fromTerm`) THEN
-  SRW_TAC [][]);
+  SRW_TAC [][]
+QED
 
 val toTerm_onto = store_thm(
   "toTerm_onto",
   ``!t. ?d. toTerm d = t``,
   METIS_TAC [fromTerm_11, fromtoTerm]);
 
-val tofromTerm = Store_thm(
-  "tofromTerm",
-  ``toTerm (fromTerm t) = t``,
-  METIS_TAC [toTerm_onto, toTerm_11, fromtoTerm])
+Theorem tofromTerm[simp] :
+    toTerm (fromTerm t) = t
+Proof
+  METIS_TAC [toTerm_onto, toTerm_11, fromtoTerm]
+QED
 
 val toTerm_eqn = store_thm(
   "toTerm_eqn",
   ``(toTerm x = y) <=> (fromTerm y = x)``,
   SRW_TAC [][EQ_IMP_THM] THEN SRW_TAC [][])
 
-val toTerm_thm = Store_thm(
-  "toTerm_thm",
-  ``(toTerm (dV i) = VAR (n2s i)) /\
+Theorem toTerm_thm[simp] :
+    (toTerm (dV i) = VAR (n2s i)) /\
     (toTerm (dAPP M N) = toTerm M @@ toTerm N) /\
-    (toTerm (dLAM i M) = LAM (n2s i) (toTerm M))``,
-  SRW_TAC [][toTerm_eqn]);
+    (toTerm (dLAM i M) = LAM (n2s i) (toTerm M))
+Proof
+  SRW_TAC [][toTerm_eqn]
+QED
 
 val lemma = prove(
   ``!i j. i + j + 1 NOTIN dFV M ==>
@@ -1029,30 +1030,34 @@ val toTerm_dABS = store_thm(
 
 val _ = overload_on ("is_dABS", ``\d. is_abs (toTerm d)``)
 
-val is_dABS_thm = Store_thm(
-  "is_dABS_thm",
-  ``(is_dABS (dV v) = F) /\
+Theorem is_dABS_thm[simp] :
+    (is_dABS (dV v) = F) /\
     (is_dABS (dAPP d1 d2) = F) /\
     (is_dABS (dABS d) = T) /\
-    (is_dABS (dLAM v d) = T)``,
+    (is_dABS (dLAM v d) = T)
+Proof
   SRW_TAC [][] THEN
   `?i N. dABS d = dLAM i N` by METIS_TAC [dABS_dLAM_exists] THEN
-  SRW_TAC [][]);
+  SRW_TAC [][]
+QED
 
-val is_dABS_vnsub_invariant = Store_thm(
-  "is_dABS_vnsub_invariant",
-  ``!d i j. is_dABS (nsub (dV i) j d) <=> is_dABS d``,
-  Induct THEN SRW_TAC [][]);
+Theorem is_dABS_vnsub_invariant[simp] :
+    !d i j. is_dABS (nsub (dV i) j d) <=> is_dABS d
+Proof
+  Induct THEN SRW_TAC [][]
+QED
 
-val is_dABS_vsub_invariant = Store_thm(
-  "is_dABS_vsub_invariant",
-  ``!d i j. is_dABS (sub (dV i) j d) <=> is_dABS d``,
-  Induct THEN SRW_TAC [][]);
+Theorem is_dABS_vsub_invariant[simp] :
+    !d i j. is_dABS (sub (dV i) j d) <=> is_dABS d
+Proof
+  Induct THEN SRW_TAC [][]
+QED
 
-val is_dABS_lift_invariant = Store_thm(
-  "is_dABS_lift_invariant",
-  ``!d j. is_dABS (lift d j) = is_dABS d``,
-  Induct THEN SRW_TAC [][]);
+Theorem is_dABS_lift_invariant[simp] :
+    !d j. is_dABS (lift d j) = is_dABS d
+Proof
+  Induct THEN SRW_TAC [][]
+QED
 
 val dbnf_def = Define`
   (dbnf (dV i) = T) /\
@@ -1061,35 +1066,41 @@ val dbnf_def = Define`
 `;
 val _ = export_rewrites ["dbnf_def"]
 
-val dbnf_vnsub_invariant = Store_thm(
-  "dbnf_vnsub_invariant",
-  ``!d i j. dbnf (nsub (dV i) j d) <=> dbnf d``,
-  Induct THEN SRW_TAC [][]);
+Theorem dbnf_vnsub_invariant[simp] :
+    !d i j. dbnf (nsub (dV i) j d) <=> dbnf d
+Proof
+  Induct THEN SRW_TAC [][]
+QED
 
-val dbnf_vsub_invariant = Store_thm(
-  "dbnf_vsub_invariant",
-  ``!d i j. dbnf (sub (dV i) j d) <=> dbnf d``,
-  Induct THEN SRW_TAC [][]);
+Theorem dbnf_vsub_invariant[simp] :
+    !d i j. dbnf (sub (dV i) j d) <=> dbnf d
+Proof
+  Induct THEN SRW_TAC [][]
+QED
 
-val dbnf_lift_invariant = Store_thm(
-  "dbnf_lift_invariant",
-  ``!d j. dbnf (lift d j) = dbnf d``,
-  Induct THEN SRW_TAC [][]);
+Theorem dbnf_lift_invariant[simp] :
+    !d j. dbnf (lift d j) = dbnf d
+Proof
+  Induct THEN SRW_TAC [][]
+QED
 
-val dbnf_dLAM = Store_thm(
-  "dbnf_dLAM",
-  ``dbnf (dLAM i d) = dbnf d``,
-  SRW_TAC [][dLAM_def]);
+Theorem dbnf_dLAM[simp] :
+    dbnf (dLAM i d) = dbnf d
+Proof
+  SRW_TAC [][dLAM_def]
+QED
 
-val dbnf_fromTerm = Store_thm(
-  "dbnf_fromTerm",
-  ``!t. dbnf (fromTerm t) = bnf t``,
-  HO_MATCH_MP_TAC simple_induction THEN SRW_TAC [][]);
+Theorem dbnf_fromTerm[simp] :
+    !t. dbnf (fromTerm t) = bnf t
+Proof
+  HO_MATCH_MP_TAC simple_induction THEN SRW_TAC [][]
+QED
 
-val bnf_toTerm = Store_thm(
-  "bnf_toTerm",
-  ``!d. bnf (toTerm d) = dbnf d``,
-  METIS_TAC [fromTerm_onto, fromtoTerm, dbnf_fromTerm]);
+Theorem bnf_toTerm[simp] :
+    !d. bnf (toTerm d) = dbnf d
+Proof
+  METIS_TAC [fromTerm_onto, fromtoTerm, dbnf_fromTerm]
+QED
 
 (* ----------------------------------------------------------------------
     Eta reduction
